HepLean.lean
@@ -121,9 +121,9 @@ import HepLean.Meta.TransverseTactics
 import HepLean.PerturbationTheory.Algebras.CrAnAlgebra.Basic
 import HepLean.PerturbationTheory.Algebras.CrAnAlgebra.NormalOrder
 import HepLean.PerturbationTheory.Algebras.CrAnAlgebra.SuperCommute
-import HepLean.PerturbationTheory.Algebras.OperatorAlgebra.Basic
-import HepLean.PerturbationTheory.Algebras.OperatorAlgebra.NormalOrder
-import HepLean.PerturbationTheory.Algebras.OperatorAlgebra.TimeContraction
+import HepLean.PerturbationTheory.Algebras.ProtoOperatorAlgebra.Basic
+import HepLean.PerturbationTheory.Algebras.ProtoOperatorAlgebra.NormalOrder
+import HepLean.PerturbationTheory.Algebras.ProtoOperatorAlgebra.TimeContraction
 import HepLean.PerturbationTheory.Algebras.StateAlgebra.Basic
 import HepLean.PerturbationTheory.Algebras.StateAlgebra.TimeOrder
 import HepLean.PerturbationTheory.CreateAnnihilate
