HepLean/PerturbationTheory/FieldSpecification/NormalOrder.lean
@@ -3,7 +3,7 @@ Copyright (c) 2025 Joseph Tooby-Smith. All rights reserved.
 Released under Apache 2.0 license as described in the file LICENSE.
 Authors: Joseph Tooby-Smith
 -/
-import HepLean.PerturbationTheory.Algebras.OperatorAlgebra.Basic
+import HepLean.PerturbationTheory.Algebras.ProtoOperatorAlgebra.Basic
 import HepLean.PerturbationTheory.Koszul.KoszulSign
 import HepLean.PerturbationTheory.FieldSpecification.Filters
 /-!
